Added concat lemmas

lib/fst/Lib.Sequence.fst
@@ -61,7 +61,7 @@ let lemma_concat3 #a len0 s0 len1 s1 len2 s2 s =
   FStar.Seq.Properties.lemma_split s (len0 + len1);
   FStar.Seq.Properties.lemma_split s' (len0 + len1)
 
-let lemma_concat4 #a len0 s0 len1 s1 len2 s2 len3 s3 s =
+let lemma_concat4_right #a len0 s0 len1 s1 len2 s2 len3 s3 s =
   let s' = concat s0 (concat s1 (concat s2 s3)) in
   FStar.Seq.Properties.lemma_split (sub s (len0 + len1) (len2 + len3)) len2;
   FStar.Seq.Properties.lemma_split (sub s' (len0 + len1) (len2 + len3)) len2;
@@ -70,7 +70,7 @@ let lemma_concat4 #a len0 s0 len1 s1 len2 s2 len3 s3 s =
   FStar.Seq.Properties.lemma_split s len0;
   FStar.Seq.Properties.lemma_split s' len0
 
-let lemma_concat5 #a len0 s0 len1 s1 len2 s2 len3 s3 len4 s4 s =
+let lemma_concat5_right #a len0 s0 len1 s1 len2 s2 len3 s3 len4 s4 s =
   let s' = concat s0 (concat s1 (concat s2 (concat s3 s4))) in
   FStar.Seq.Properties.lemma_split (sub s (len0 + len1 + len2) (len3 + len4)) len3;
   FStar.Seq.Properties.lemma_split (sub s' (len0 + len1 + len2) (len3 + len4)) len3;
